Almost working

src/dup.v
@@ -33,6 +33,26 @@ Section inductive_predicate_strictly_sorted.
     destruct H; auto with strictly_sorted.
   Qed.
 
+  Local Ltac extract_info_from_strictly_sorted :=
+    unfold not; intros; subst;
+    match goal with
+    | [ H: is_strictly_sorted (?x0 :: ?xs) |- _ ]
+      => inversion H; subst;
+         try discriminate (* this eliminates some impossible cases *)
+    end;
+    destruct_list_equality.
+
+  Lemma is_strictly_sorted_implies_sorted: forall (ls : list A),
+      is_strictly_sorted ls -> is_sorted ls.
+  Proof.
+    induction ls.
+    - constructor.
+    - extract_info_from_strictly_sorted.
+      + constructor.
+      + constructor. left. assumption.
+        apply IHls. assumption.
+  Qed.
+
   Local Ltac is_strictly_sorted_contradiction_via_tail :=
     match goal with
     | [ H: is_strictly_sorted (?x0 :: ?xs),
@@ -52,14 +72,6 @@ Section inductive_predicate_strictly_sorted.
   Definition is_strictly_sorted_dec: forall (ls :list A),
       {is_strictly_sorted ls} + {~(is_strictly_sorted ls)}.
 
-    Local Ltac extract_info_from_strictly_sorted :=
-      unfold not; intros; subst;
-      match goal with
-      | [ H: is_strictly_sorted (?x0 :: ?xs) |- _ ]
-        => inversion H; subst;
-           try discriminate (* this eliminates some impossible cases *)
-      end;
-      destruct_list_equality.
 
     refine (
         fix F (ls: list A) : {is_strictly_sorted ls} + {~(is_strictly_sorted ls)} :=
@@ -100,6 +112,192 @@ End inductive_predicate_strictly_sorted.
 Section remove_duplicates_from_sorted.
   Context {A: Type}.
   Context {cmp: comparable A}.
+
+  (* HELP WANTED: isn't there some library that more or less does this?
+   The ones I found don't seem to have a notation of equality of sets. *)
+  Definition list_set_eq (xs ys : list A): Prop :=
+    forall (a : A), (In a xs) <-> (In a ys).
+
+  Hint Unfold list_set_eq: list_set_db.
+  Hint Extern 0 (_ <-> _) => split : list_set_db.
+
+  Lemma list_set_eq_refl (xs: list A):
+    list_set_eq xs xs.
+  Proof.
+    auto with list_set_db.
+  Qed.
+
+  Hint Resolve list_set_eq_refl: list_set_db.
+
+  Lemma list_set_eq_symm (xs ys: list A):
+    list_set_eq xs ys <-> list_set_eq ys xs.
+  Proof.
+    (* QUESTION: why can't auto do this? *)
+    split;
+      intro H;
+      unfold list_set_eq in *;
+      intro;
+      split; apply H.
+  Qed.
+
+  Lemma list_set_eq_step (a : A) (xs: list A):
+    list_set_eq (a::xs) (a::(a::xs)).
+  Proof.
+    autounfold with list_set_db.
+    intros.
+    split.
+    - intro H.
+      unfold In.
+      destruct (compare_eq_dec a a0); auto.
+    - intro H.
+      unfold In.
+      (* Here auto doesn't work, because we need to destruct H twice
+       (one time we do it manually; one time, it happens in auto).
+       Is there some way we can add that as a kind of hint? *)
+      destruct (compare_eq_dec a a0).
+      + auto.
+      + unfold In in H.
+        destruct H; auto.
+  Qed.
+
+  Lemma list_set_eq_trans (xs ys zs : list A):
+    list_set_eq xs ys
+    -> list_set_eq ys zs
+    -> list_set_eq xs zs.
+  Proof.
+    intros.
+    unfold list_set_eq in *.
+    intro.
+    split.
+    - intro.
+      auto using H, H0 with list_set_db.
+      (* QUESTION: how can the above auto statement fail to just apply the hints I told it to apply? *)
+      apply H0.
+      apply H.
+      assumption.
+    - intro.
+      apply H.
+      apply H0.
+      assumption.
+  Qed.
+
+  Lemma list_set_eq_ind_step (xs ys: list A) (x : A):
+    list_set_eq xs ys ->
+    list_set_eq (x::xs) (x::ys).
+  Proof.
+    intros.
+    unfold list_set_eq.
+    intros.
+    split.
+    - intros H0.
+      destruct H0.
+      + subst. cbn. auto.
+      + subst. cbn. right.
+        apply H. assumption.
+    - intros H0.
+      destruct H0.
+      + subst. cbn. auto.
+      + subst. cbn. right.
+        apply H. assumption.
+  Qed.
+
+  (* The result has to satisfy two properties:
+1. It is strictly sorted.
+2. As a set, it is equal to the input.
+   *)
+  Fixpoint remove_duplicates_from_sorted (ls : list A):
+    is_sorted ls ->
+    { lres : list A | is_strictly_sorted lres & list_set_eq ls lres }.
+    intros.
+    destruct ls as [| a0 ls'] eqn:?.
+    - subst.
+      refine (exist2 _ _ [] _ _).
+      + constructor.
+      + apply list_set_eq_refl.
+    - assert (is_sorted ls') as Hls'sorted.
+      apply tail_of_is_sorted_is_sorted with (x := a0).
+      assumption.
+
+      pose (remove_duplicates_from_sorted ls' Hls'sorted) as res.
+
+      destruct ls' as [| a1 ls''] eqn:?.
+
+      + refine (exist2 _ _ ls _ _).
+        subst. constructor. subst.
+        apply list_set_eq_refl.
+      + destruct (compare a0 a1) eqn:?.
+        * (* Case: a0 = a1 *)
+          refine (exist2 _ _
+                         (proj1_sig (sig_of_sig2 res))
+                         (proj2_sig (sig_of_sig2 res))
+                         _).
+
+          apply list_set_eq_trans with
+              (xs := (a0 :: a1 :: ls''))
+              (ys := ls')
+              (zs := (proj1_sig (sig_of_sig2 res))).
+          subst. compare_to_eq. subst.
+          apply list_set_eq_symm.
+          apply list_set_eq_step with (a := a1)
+                                      (xs := (ls'')).
+
+          subst.
+          exact (proj3_sig res).
+
+        * (* Case: a0 < a1 *)
+          set (res_list :=
+                 (proj1_sig (sig_of_sig2 res))).
+
+          refine (exist2 _ _
+                         (a0 :: res_list)
+                         _ _).
+
+          -- (* proof of strictly sorted *)
+             destruct res_list as [| res0 res_list' ] eqn:?; try constructor.
+             subst.
+
+             assert (compare_leq a1 res0).
+             (* Will use: a1 in  (a1 :: ls''), which is sorted;
+              res0 is also in there *)
+             assert (In res0 (a1 :: ls'')).
+             apply (proj3_sig res).
+             replace (proj1_sig (sig_of_sig2 res)) with res_list.
+             rewrite Heql1.
+             cbn. auto. auto.
+
+             replace a1 with (hd a1 (a1 :: ls'')).
+             apply is_sorted_first_element_smallest.
+             apply tail_of_is_sorted_is_sorted with (x := a0).
+             assumption.
+
+             assumption.
+             auto.
+
+             (* now use transitivity *)
+             apply compare_lt_leq_trans with (y := a1);
+             assumption.
+
+             subst.
+             rewrite <- Heql1.
+             exact (proj2_sig (sig_of_sig2 res)).
+
+          -- (* proof of list equality *)
+            (* idea of proof: both have a0; and the rest
+            of the list is equal by recursion. *)
+            apply list_set_eq_ind_step.
+            unfold res_list.
+            subst.
+            exact (proj3_sig res).
+
+        * (* Case a0 > a1; contradiction *)
+          exfalso.
+          remember (first_two_of_is_sorted_are_sorted H) as Hcontrad.
+          destruct Hcontrad; contradiction_from_compares.
+  Defined.
+
+
+
+
 
   (* The type of this function does not entirely specify the function: the
      result may be a strictly sorted list, but there is nothing that says it is
